src/coq/Classes.v
@@ -485,11 +485,3 @@ Fixpoint to_string_b10' fuel (x:Z) : string :=
 Definition to_string_b10 := to_string_b10' 10000.
 
 Instance string_of_Z : StringOf Z := to_string_b10.
-
-
-
-
-
-
-
-
